Rustv/Tests/ex/SharedWrite.thy
@@ -63,13 +63,11 @@ text \<open>Proof of safety (the program doesn't stuck due to alias semantics vi
 lemma "\<Gamma> \<turnstile>\<^sub>t {s. wf_heap s} shared_body {s. True}"
   unfolding shared_body_def
   apply vcg
-  apply (auto simp add: Let_def wf_tags_spec)
-  sorry
+  by (auto simp add: Let_def wf_tags_spec)
 
 lemma "\<Gamma> \<turnstile>\<^sub>t {s. wf_heap s} shared_body {s. wf_heap s}"
   unfolding shared_body_def
   apply vcg
-  apply (auto simp add: Let_def wf_tags_spec)
-  sorry
+  by (auto simp add: Let_def wf_tags_spec)
 
 end
